TaplLean/STLC/Termination.lean
@@ -1,0 +1,237 @@
+import Mathlib.Logic.Relation
+import TaplLean.STLC.Env
+
+inductive Type_ where
+  | TBase : Type_
+  | TArrow : Type_ → Type_ → Type_
+open Type_
+
+abbrev TyEnv := Env Type_
+
+inductive Term_ where
+  | var : String → Term_
+  | abs : String → Type_ → Term_ → Term_
+  | app : Term_ → Term_ → Term_
+open Term_
+
+infixr:50 " :-> " => Type_.TArrow
+notation:90 "λ" x " : " T " , " t => Term_.abs x T t
+
+def subst (x : String) (s : Term_) (t : Term_) :=
+  match t with
+  | var y       => if x = y then s else t
+  | λ y : T, t' => if x = y then t else λ y : T, subst x s t'
+  | app t1 t2   => app (subst x s t1) (subst x s t2)
+
+inductive WellTyped : TyEnv → Term_ → Type_ → Prop where
+  | wt_var : ∀ {Γ x T}, Γ x = some T → WellTyped Γ (var x) T
+  | wt_abs : ∀ {Γ x t1 T1 T2},
+      WellTyped (x |→ T2; Γ) t1 T1 →
+      WellTyped Γ (λ x : T2 , t1) (T2 :-> T1)
+  | wt_app : ∀ {Γ t1 t2 T1 T2},
+      WellTyped Γ t1 (T2 :-> T1) →
+      WellTyped Γ t2 T2 →
+      WellTyped Γ (app t1 t2) T1
+open WellTyped
+
+notation:20 "[" x " := " s " ] " t => subst x s t
+notation:100 Γ " ⊢ " t " ∈: " T => WellTyped Γ t T
+
+theorem weakening : ∀ {Γ Γ' t T},
+  includeIn Γ Γ' →
+  (Γ ⊢ t ∈: T) → Γ' ⊢ t ∈: T
+  := by
+  intro Γ Γ' t T Hin HT
+  revert Γ'
+  induction HT
+  case wt_var Δ x U HD =>
+    intro Δ' Hin
+    simp [includeIn] at Hin
+    have Hin' := Hin x U HD
+    apply wt_var Hin'
+  case wt_abs Δ x t1 T1 T2 HT IH =>
+    intro Δ' Hin
+    have Hin_ext := update_includeIn x T2 Hin
+    have HT_G' := IH Hin_ext
+    apply wt_abs HT_G'
+  case wt_app Δ t1 t2 T1 T2 HT_fun HT_arg IH_fun IH_arg =>
+    intro Δ' Hin
+    apply wt_app (IH_fun Hin) (IH_arg Hin)
+  done
+
+theorem weakening_empty : ∀ {t T} (Γ),
+  (empty ⊢ t ∈: T) → Γ ⊢ t ∈: T
+  := by
+  intro t T Γ H
+  have Hin := empty_min Γ
+  apply weakening Hin H
+  done
+
+inductive Value : Term_ → Prop where
+  | v_abs : ∀ {x T t}, Value (λx:T, t)
+
+inductive Step : Term_ → Term_ → Prop where
+  | st_app_abs : ∀ {x T2 t1 v2},
+      Value v2 →
+      Step (app (λx:T2,t1) v2) ([x := v2] t1)
+  | st_app1 : ∀ {t1 t1' t2},
+      Step t1 t1' →
+      Step (app t1 t2) (app t1' t2)
+  | st_app2 : ∀ {v1 t2 t2'},
+      Value v1 →
+      Step t2 t2' →
+      Step (app v1 t2) (app v1 t2')
+notation:40 t " -> " t' => Step t t'
+open Step
+
+def stepStar := Relation.ReflTransGen Step
+notation:40 t " -*> " t' => stepStar t t'
+
+def terminate (t : Term_) := ∃ t', (t -*> t') ∧ Value t'
+
+-- inductive R : Type_ → Term_ → Prop where
+--   | R_base : ∀ {T t},
+--       (empty ⊢ t ∈: T) →
+--       terminate t →
+--       R T t
+--   | R_arrow : ∀ {T1 T2 t},
+--       (empty ⊢ t ∈: T1 :-> T2) →
+--       terminate t →
+--       (∀ s, R T1 s → R T2 (app t s)) →
+--       R (T1 :-> T2) t
+
+def R (T : Type_) (t : Term_) : Prop :=
+  match T with
+  | TBase => (empty ⊢ t ∈: T) ∧ terminate t
+  | TArrow T1 T2 =>
+      (empty ⊢ t ∈: T1 :-> T2) ∧
+      terminate t ∧
+      (∀ s, R T1 s → R T2 (app t s))
+
+theorem R_term_is_terminate : ∀ {T t}, R T t → terminate t
+  := by
+  intro T t H_R
+  cases T
+  case TBase =>
+    simp [R] at H_R
+    apply H_R.right
+  case TArrow T1 T2 =>
+    simp [R] at H_R
+    apply H_R.right.left
+  done
+
+-- 書換えにより危険対は生じない
+theorem step_deterministic : ∀ {t t' t'' : Term_},
+  (t -> t') → (t -> t'') → t' = t''
+  := by
+  intro t t' t'' H1 H2
+  revert t''
+  induction H1
+  case st_app_abs x T2 t1 v2 H_v2 =>
+    intro t'' H_st
+    cases H_st
+    case st_app_abs =>
+      trivial
+    case st_app1 _ Contra =>
+      cases Contra
+    case st_app2 _ _ Contra =>
+      cases H_v2
+      cases Contra
+  case st_app1 t1 t1' t2 H_st1 IH =>
+    intro t'' H_st_app
+    cases H_st_app
+    case st_app_abs =>
+      cases H_st1
+    case st_app1 t1'' H_t1 =>
+      have H_eq' := IH H_t1
+      rw [H_eq']
+    case st_app2 t2' H_v1 H_st2 =>
+      cases H_v1
+      cases H_st1
+  case st_app2 v1 t2 t2' H_v1 H_st2 IH =>
+    intro u H
+    cases H_v1
+    cases H
+    case st_app_abs _ _ _ H_v2 =>
+      cases H_v2
+      cases H_st2
+    case st_app1 _ _ _ Contra =>
+      cases Contra
+    case st_app2 x T t t2'' HV_t H_st2' =>
+      have H_eq2 := IH H_st2'
+      rw [H_eq2]
+  done
+
+theorem step_preserve_termination : ∀ {t t' : Term_},
+  (t -> t') → (terminate t ↔ terminate t')
+  := by
+  intro t t' H_st
+  simp [terminate]
+  apply Iff.intro
+  . -- * → *
+    intro H_t
+    cases H_t; rename_i u H_u
+    induction H_u.left using Relation.ReflTransGen.head_induction_on
+    case refl =>
+      cases H_u.right
+      cases H_st
+    case head a b Hst_ab Hmst IH =>
+      have Heq := step_deterministic Hst_ab H_st
+      rw [Heq] at Hmst
+      exists u
+      apply And.intro Hmst H_u.right
+  . -- * ← *
+    intro H_t'
+    cases H_t'; rename_i u' H
+    induction H.left using Relation.ReflTransGen.head_induction_on
+    case refl =>
+      exists u'
+      apply And.intro (Relation.ReflTransGen.single H_st) H.right
+    case head a _ _ _ _ =>
+      have Hmst := Relation.ReflTransGen.head H_st H.left
+      exists u'
+      apply And.intro Hmst H.right
+  done
+
+theorem substitution_preserve_type : ∀ {Γ x S t T s},
+  ((x |→ S; Γ) ⊢ t ∈: T) →
+  (empty ⊢ s ∈: S) →
+  Γ ⊢ ([x := s] t) ∈: T
+  := by
+  intro Γ x S t T s
+  revert Γ T
+  induction t <;> intro Γ T HT_t HT_s
+  case var =>
+    rename_i y
+    simp [subst]
+    cases String.decEq x y
+    case isFalse Hneq =>
+      unfold update at HT_t; cases HT_t; rename_i HT_t
+      simp [Hneq] at HT_t
+      simp [Hneq]
+      apply wt_var HT_t
+    case isTrue Heq =>
+      unfold update at HT_t; cases HT_t; rename_i HT_t
+      simp [Heq] at HT_t
+      simp [Heq]
+      have HT_s := weakening_empty Γ HT_s
+      rw [← HT_t]
+      assumption
+
+theorem step_preserve_type : ∀ {t t' : Term_} {T : Type_},
+  (t -> t') → (empty ⊢ t ∈: T) → (empty ⊢ t' ∈: T)
+  := by
+  intro t t' T Hst HT_t
+  induction Hst
+  case st_app_abs x T2 t1 v2 H_v2 =>
+    apply wt_app
+
+theorem step_preserve_R : ∀ {T t t'},
+  (empty ⊢ t ∈: T) →
+  (t -> t') →
+  (R T t ↔ R T t')
+  := by
+  intro T t t' H_st HR
+  induction T <;> apply Iff.intro
+  case TBase =>
+    simp [R]
