lakefile.lean
@@ -11,4 +11,5 @@ lean_lib «TaplLean» where
 lean_exe «tapl-lean» where
   root := `Main
 
-require batteries from git "https://github.com/leanprover-community/batteries" @ "main"
+require batteries from git "https://github.com/leanprover-community/batteries" @ "v4.10.0"
+require mathlib from git "https://github.com/leanprover-community/mathlib4" @ "v4.10.0"
